Matroids/Sort.lean
@@ -1,0 +1,9 @@
+import Mathlib.Data.List.Sort
+-- import Mathlib.Data.List.Lex
+
+-- variable {X : Type*} [LT X] [DecidableRel ((·:X) < · )] [BEq X ]
+/-- Function that sorts, outside PartialMatroid namespace. It will sort lists by dtermining which
+list is greater. Its criteria for determining the greater list is whichever list generates a greater
+number first-/
+def List.sort {X : Type*} [LinearOrder X] (l : List X) : List X :=
+   l.mergeSort (· < · )
