Matroids/Verification/Miscellaneous.lean
@@ -67,131 +67,15 @@ lemma List.Forall.join {L : List (List α)} {P : α → Prop} (hl : L.Forall fun
     constructor
     · exact th1
     · exact h1
-
-lemma List.mem_mergeSort (r : α → α → Prop) [h: DecidableRel r] {l : List α} (h : a ∈ l) :
-    a ∈ l.mergeSort r := by
-  rw [List.Perm.mem_iff]
-  · apply h
-  · apply List.perm_mergeSort
-
-lemma List.reverse_mem_mergeSort (r : α → α → Prop) [h: DecidableRel r] {l : List α} (h : a ∈ l.mergeSort r) :
-    a ∈ l := by
-  rw [List.Perm.mem_iff]
-  · apply h
-  · apply List.Perm.symm
-    apply List.perm_mergeSort
-
-lemma List.not_mem_mergeSort (r : α → α → Prop) [h: DecidableRel r] {l : List α} (h : a ∉ l) :
-    a ∉ l.mergeSort r := by
-  rw [List.Perm.mem_iff]
-  · apply h
-  · apply List.perm_mergeSort
-
-lemma List.forall_mergeSort (r : α → α → Prop) [h: DecidableRel r] {l : List α} {P : α → Prop }
-    (h1 : l.Forall P) : (l.mergeSort (r)).Forall P := by
-  rw [List.forall_iff_forall_mem]
-  intro i hi
-  rw [List.forall_iff_forall_mem] at h1
-  apply h1
-  rw [List.Perm.mem_iff]
-  apply hi
-  apply List.Perm.symm
-  apply List.perm_mergeSort
-
-
-lemma List.split_of_sublist {l : List α} :
-    List.Sublist (l.split).1 l ∧ List.Sublist (l.split).2 l:= by
-  match l with
-  | [] => simp
-  | a :: l =>
-    unfold split
-    simp
-    have ih := @List.split_of_sublist l
-    constructor
-    · apply List.Sublist.cons_cons
-      exact ih.2
-    · apply List.sublist_cons_of_sublist
-      exact ih.1
-
-
-/- Paused for the moment, we will focus on proving sorted_mergeSort for the less than relationship-/
-lemma List.mergeSort_lt_eq_mergeSort_le [LinearOrder α] {l : List α}
-    (h_nodup : l.Nodup):
-    mergeSort (· < ·) l = mergeSort (· ≤ ·) l  := by
-  match l with
-  | [] => simp
-  | [a] => simp
-  | a :: b :: l =>
-    unfold mergeSort
-    simp
-    have ha1 : List.Sublist (a :: (split l).1) (a :: b :: l) := by
-      apply List.Sublist.cons_cons
-      apply List.sublist_cons_of_sublist
-      apply List.split_of_sublist.1
-    have hb2 : List.Sublist (b :: (split l).2) (a :: b :: l) := by
-      apply List.sublist_cons_of_sublist
-      apply List.Sublist.cons_cons
-      apply List.split_of_sublist.2
-    have ha := List.Nodup.sublist ha1 h_nodup
-    have hb := List.Nodup.sublist hb2 h_nodup
-    -- have iha := List.mergeSort_lt_eq_mergeSort_le ha
-    -- have ihb := List.mergeSort_lt_eq_mergeSort_le hb
-    -- simp_rw[iha,ihb]
-    -- unfold merge
-    -- have : (split l = ((split l).1, (split l).2)) := by simp
-    -- have := perm_split this
-
-    -- simp at h_nodup
-    -- obtain ⟨hab, _, _⟩ := h_nodup
-    -- rw[or_iff_not_and_not] at hab
-    -- simp at hab
-    -- match mergeSort (fun x x_1 => x ≤ x_1) (a :: (split l).1), mergeSort (fun x x_1 => x ≤ x_1) (b :: (split l).2) with
-    -- | [], [] => simp
-    -- | [], l' => simp
-    -- | a :: l, [] => simp
-    -- | (x1 :: l1 as full1), (x2 :: l2 as full2)=>
-    --   simp
-
-    -- conv =>
-    --   lhs
-    --   arg 6
-    --   intro x1 x2 x3 x4
-      -- rw[lt_iff_le_and_ne (a := x1) (b := x3)]
-
-    sorry
-
 #check List.Nodup.sublist
 #check List.split
 #check lt_iff_le_and_ne
-
-/--mergeSort with the less than relation has no duplicates-/ -- Wrong lemma, counterexample below
-lemma List.mergeSort_no_duplicates [PartialOrder α] {l : List α} [DecidableRel ((· : α) < ·)]:
-   Nodup (mergeSort (· < ·) l) :=
-
-  sorry
-
-#eval mergeSort (· < ·) [1,1,2]
-
 
 theorem List.pairwise_range {R : ℕ → ℕ → Prop} (H : ∀ i j, i < j → R i j) :
     List.Pairwise R (List.range n) := by
   apply @List.Pairwise.imp Nat (fun a b => a < b) R
   · apply H
   · exact pairwise_lt_range n
-
-/- PENDING theorem: If you have two different sorted lists and you run merge on them,
-then the result has to be sorted. Take a look at theorem Sorted.merge-/
-
-
-theorem sorted_mergeSort_lt [PartialOrder α] {l : List α} [DecidableRel ((· : α) < ·)] :
-    ∀ l : List α, Sorted (· < ·) (mergeSort (· < ·) l)
-  | [] => by simp [mergeSort]
-  | [a] => by simp [mergeSort]
-  | a :: b :: l => by
-    simp [mergeSort]
-
-    sorry
-
 -- in the file Init.Data.List.Sublist
 -- added in https://github.com/leanprover/lean4/pull/5053, August 2024
 theorem List.Sublist.mem {α : Type*} {l₁ : List α} {a : α} {l₂ : List α} (hx : a ∈ l₁)
@@ -204,9 +88,4 @@ lemma List.Forall.perm {L₁ L₂ :List X} {P : X → Prop } (hL : L₁.Perm L�
     (hp: L₁.Forall P) :
     L₂.Forall P := by
   -- apply?
-  sorry
-
-
-lemma mergeSort_of_perm_eq {L₁ L₂ : List X} (P : X → X → Prop) [DecidableRel P] (hL : L₁.Perm L₂) :
-    List.mergeSort P L₁ = List.mergeSort P L₂ := by
   sorry
