Matroids/Verification/Sort.lean
@@ -1,0 +1,153 @@
+import Matroids.Sort
+import Mathlib.Data.List.Lex
+import Mathlib.Data.List.Sort
+
+
+open List
+
+/--mergeSort with the less than relation has no duplicates-/ -- Wrong lemma, counterexample below
+lemma List.mergeSort_no_duplicates [PartialOrder α] {l : List α} [DecidableRel ((· : α) < ·)]:
+   Nodup (mergeSort (· < ·) l) :=
+
+  sorry
+
+#eval mergeSort (· < ·) [1,1,2]
+
+
+
+lemma List.split_of_sublist {α : Type*} {l : List α} :
+    List.Sublist (l.split).1 l ∧ List.Sublist (l.split).2 l:= by
+  match l with
+  | [] => simp
+  | a :: l =>
+    unfold split
+    simp
+    have ih := List.split_of_sublist (l := l)
+    constructor
+    · apply List.Sublist.cons_cons
+      exact ih.2
+    · apply List.sublist_cons_of_sublist
+      exact ih.1
+
+
+/- Paused for the moment, we will focus on proving sorted_mergeSort for the less than relationship-/
+lemma List.mergeSort_lt_eq_mergeSort_le [LinearOrder α] {l : List α}
+    (h_nodup : l.Nodup):
+    mergeSort (· < ·) l = mergeSort (· ≤ ·) l  := by
+  match l with
+  | [] => simp
+  | [a] => simp
+  | a :: b :: l =>
+    unfold mergeSort
+    simp
+    have ha1 : List.Sublist (a :: (split l).1) (a :: b :: l) := by
+      apply List.Sublist.cons_cons
+      apply List.sublist_cons_of_sublist
+      apply List.split_of_sublist.1
+    have hb2 : List.Sublist (b :: (split l).2) (a :: b :: l) := by
+      apply List.sublist_cons_of_sublist
+      apply List.Sublist.cons_cons
+      apply List.split_of_sublist.2
+    have ha := List.Nodup.sublist ha1 h_nodup
+    have hb := List.Nodup.sublist hb2 h_nodup
+    -- have iha := List.mergeSort_lt_eq_mergeSort_le ha
+    -- have ihb := List.mergeSort_lt_eq_mergeSort_le hb
+    -- simp_rw[iha,ihb]
+    -- unfold merge
+    -- have : (split l = ((split l).1, (split l).2)) := by simp
+    -- have := perm_split this
+
+    -- simp at h_nodup
+    -- obtain ⟨hab, _, _⟩ := h_nodup
+    -- rw[or_iff_not_and_not] at hab
+    -- simp at hab
+    -- match mergeSort (fun x x_1 => x ≤ x_1) (a :: (split l).1), mergeSort (fun x x_1 => x ≤ x_1) (b :: (split l).2) with
+    -- | [], [] => simp
+    -- | [], l' => simp
+    -- | a :: l, [] => simp
+    -- | (x1 :: l1 as full1), (x2 :: l2 as full2)=>
+    --   simp
+
+    -- conv =>
+    --   lhs
+    --   arg 6
+    --   intro x1 x2 x3 x4
+      -- rw[lt_iff_le_and_ne (a := x1) (b := x3)]
+
+    sorry
+
+
+lemma List.mem_mergeSort (r : α → α → Prop) [h: DecidableRel r] {l : List α} (h : a ∈ l) :
+    a ∈ l.mergeSort r := by
+  rw [List.Perm.mem_iff]
+  · apply h
+  · apply List.perm_mergeSort
+
+lemma List.reverse_mem_mergeSort (r : α → α → Prop) [h: DecidableRel r] {l : List α} (h : a ∈ l.mergeSort r) :
+    a ∈ l := by
+  rw [List.Perm.mem_iff]
+  · apply h
+  · apply List.Perm.symm
+    apply List.perm_mergeSort
+
+lemma List.not_mem_mergeSort (r : α → α → Prop) [h: DecidableRel r] {l : List α} (h : a ∉ l) :
+    a ∉ l.mergeSort r := by
+  rw [List.Perm.mem_iff]
+  · apply h
+  · apply List.perm_mergeSort
+
+lemma List.forall_mergeSort (r : α → α → Prop) [h: DecidableRel r] {l : List α} {P : α → Prop }
+    (h1 : l.Forall P) : (l.mergeSort (r)).Forall P := by
+  rw [List.forall_iff_forall_mem]
+  intro i hi
+  rw [List.forall_iff_forall_mem] at h1
+  apply h1
+  rw [List.Perm.mem_iff]
+  apply hi
+  apply List.Perm.symm
+  apply List.perm_mergeSort
+
+
+
+/- PENDING theorem: If you have two different sorted lists and you run merge on them,
+then the result has to be sorted. Take a look at theorem Sorted.merge-/
+
+
+theorem sorted_mergeSort_lt [PartialOrder α] {l : List α} [DecidableRel ((· : α) < ·)] :
+    ∀ l : List α, Sorted (· < ·) (mergeSort (· < ·) l)
+  | [] => by simp [mergeSort]
+  | [a] => by simp [mergeSort]
+  | a :: b :: l => by
+    simp [mergeSort]
+
+    sorry
+
+
+
+lemma sort_map_sort {L : List X} [LinearOrder X] {f: X → X}:
+    List.sort ( List.map f L.sort) = List.sort (List.map f L) := by
+  sorry
+
+lemma sort_join_sort {X :Type} [LinearOrder X] (L : List (List X)) :
+    List.sort (List.join (List.sort L)) = List.sort (List.join (L)) := by
+  match L with
+  |[] => simp
+  |a :: ll =>
+    simp
+    have h := sort_join_sort ll
+    match a with
+    |[] =>
+      simp
+      sorry
+    |c :: l =>
+      sorry
+-- proof idea: consider number of occurence in each list, should be the same
+
+lemma sort_join_map_sort {X : Type} [LinearOrder X] (L : List (List X)):
+    List.sort (List.join (List.map List.sort L)) = List.sort (List.join (L)) := by
+  sorry
+
+
+lemma mergeSort_of_perm_eq {L₁ L₂ : List X} (P : X → X → Prop) [DecidableRel P] (hL : L₁.Perm L₂) :
+    List.mergeSort P L₁ = List.mergeSort P L₂ := by
+  sorry
